\documentclass{article}
\usepackage[skip=10pt]{parskip}
\usepackage{amsmath}
\usepackage{amssymb}
\begin{document}

3a. Let's consider the expression $n!e^n$.

\[ n!e^n = \prod_{k=1}^n ke \]

We are now going to replace each of the $e$'s with an inequality based on the fact that $e > (1 + 1 / r)^r$ for all positive integers $r$.

\begin{align*}
    n!e^n &> \prod_{k=1}^n k(1 + 1 /k)^k \\
    n!e^n &> \prod_{k=1}^n (k + 1)^k / k^{k - 1}
\end{align*}

We can now cancel each of the denominators on the RHS with the preceding numerator, and obtain

\begin{align*}
    n!e^n &> (n + 1)^n \\
    n!e^n &> n^n \\
    \therefore n! &> (n / e)^n
\end{align*}

This concludes the proof.

\end{document}
